$$
\begin{split}
{\theta}''_{1}&=-\omega_{0}^{2} \theta_{1} - \gamma \theta_1'-k\left(\theta_{1}-\theta_{2}\right) \\ 
{\theta}''_{2}&=-\omega_{0}^{2} \theta_{2} - \gamma \theta_2'-k\left(\theta_{2}-\theta_{1}\right)-k\left(\theta_{2}-\theta_{3}\right) \\ 
{\theta}''_{3}&=-\omega_{0}^{2} \theta_{3} - \gamma \theta_3' -k\left(\theta_{3}-\theta_{2}\right) 
\end{split} 
$$

Define $u_i = \theta_i$ and $v_i = \theta_i'$. 

$$
\begin{split}
u_1' &=  v_1 \\ 
u_2' &= v_2 \\ 
u_3' &= v_3 \\ 
v'_{1} &=-\omega_{0}^{2} u_{1} - \gamma v_1 -k\left(u_{1}-u_{2}\right) \\ 
v'_{2} &=-\omega_{0}^{2} u_{2}- \gamma v_2-k\left(u_{2}-u_{1}\right)-k\left(u_{2}-u_{3}\right) \\ 
v'_{3} &=-\omega_{0}^{2} u_{3}- \gamma v_3-k\left(u_{3}-u_{2}\right) 
\end{split} 
$$
